reorganising machine section to be easier to instantiate

proof/Merges/Machine/Id.v
@@ -1,6 +1,9 @@
 Require Import Merges.Machine.Machine.
 Require Import Merges.Map.
-Set Implicit Arguments.
+
+(* It's actually somewhat nicer without this.
+   Seems that inference for record values isn't so good. *)
+(* Set Implicit Arguments. *)
 
 Require Import Merges.List.List.
 Require Import Coq.Lists.List.
@@ -10,32 +13,65 @@ Require Import Coq.Program.Equality.
 
 Require Import Merges.Tactics.
 
+(* Let's define a simple machine *)
+
+
+(* With one input *)
 Inductive Input := Input_.
+
 Theorem InputEqDec : EqDec Input.
+Proof.
  unfold EqDec.
  intros.
  destruct n; destruct m; eauto.
 Qed.
 
+(* And one output *)
 Inductive Output := Output_.
+
 Theorem OutputEqDec : EqDec Output.
  unfold EqDec.
  intros.
  destruct n; destruct m; eauto.
 Qed.
 
-Definition Val := nat.
+(* Which only works over nats *)
+Definition val := nat.
+Definition uninitialised : val := 0.
 
+(* And has three states *)
 Inductive Label
  := L0 | L1 | L2.
 
-Definition stateOf (l : Label) : State Input Output Val Label
+Definition IdTypes
+ := mkTypes
+    InputEqDec
+    OutputEqDec
+    uninitialised
+    L0.
+
+(* Repeatedly pull from input, writing to output *)
+Definition stateOf (l : Label) : State IdTypes
  := match l with
-    | L0 => Pull _ _ Input_  L1 L2
-    | L1 => Out  Output_ (fun e => e (VInput _ Input_)) L0
-    | L2 => Done _ _ _ _
+    | L0 => Pull IdTypes Input_  L1 L2
+    | L1 => @Out IdTypes Output_ (fun e => e (VInput IdTypes Input_)) L0
+    | L2 => Done IdTypes
     end.
 
+(* Does it terminate for all states? *)
+(*
+Lemma termination_all: @terminates_all_states IdTypes stateOf.
+Proof.
+ unfold terminates_all_states.
+ intros.
+ repeat eexists.
+ destruct l.
+ eapply Exec.
+ simpl.
+ apply Run1.
+ constructor.
+ eauto.
+*)
 (*Theorem Exec: forall (inp : list nat) (os : Outputs Output nat),
     exec InputEqDec OutputEqDec 0 L0 stateOf (fun _ => inp) os
  -> os Output_ = reverse inp.
