proof/Merges/Machine/Machine.v
@@ -7,99 +7,110 @@ Set Implicit Arguments.
 
 Section Machine.
 
- (* ~~~~ Definition ~~~~~~~~ *)
+ (* ~~~~ Input types ~~~~~~~~ *)
+ Record Types
+  := mkTypes
 
- (* The names of input channels *)
- Variable   input       : Type.
- (* do we need to see if two are the same? *)
- Hypothesis inputEqDec  : EqDec input.
+  (* The names of input channels *)
+  { input       : Type
+  (* do we need to see if two are the same? *)
+  ; inputEqDec  : EqDec input
 
- (* The names of output channels.
-    I'm not sure whether separating these will make fusion too complicated
-    because fusing can remove inputs  *)
- Variable   output      : Type.
- (* do we need to see if two are the same? *)
- Hypothesis outputEqDec : EqDec output.
+  (* The names of output channels.
+     I'm not sure whether separating these will make fusion too complicated
+     because fusing can remove inputs  *)
+  ; output      : Type
+  (* do we need to see if two are the same? *)
+  ; outputEqDec : EqDec output
+
+  (* Let's start simple with only one value type *)
+  ; val         : Type
+  (* And we'll assume there is some sort of bottom for uninitialised values.
+     This is not ideal, but it makes it simpler to allow worker functions
+     access to all values *)
+  ; uninitialised : val
+
+  (* State labels *)
+  ; label       : Type
+  (* We also need an initial label *)
+  ; initial     : label
+
+  (* The stateOf : label -> State
+     would make sense in here, but State isn't defined yet
+     and depends on the types in here *)
+  }.
+
+ Variable t : Types.
 
 
- (* Let's start simple with only one value type *)
- Variable   val   : Type.
- (* And we'll assume there is some sort of bottom for uninitialised values.
-    This is not ideal, but it makes it simpler to allow worker functions
-    access to all values *)
- Variable   uninitialised : val.
 
+ (* ~~~~ Definitions ~~~~~~~~ *)
 
  (* Output channels can have states assigned to them.
     You can also read the last output value. *)
  Inductive Var
    (* Value of last read from channel *)
-  := VInput       : input  -> Var
+  := VInput       : input  t -> Var
    (* Value that was last written to channel *)
-   | VOutput      : output -> Var
+   | VOutput      : output t -> Var
    (* Output channel's state *)
-   | VState       : output -> Var.
+   | VState       : output t -> Var.
 
  Theorem VarEqDec : EqDec Var.
   unfold EqDec in *. intros.  
   destruct n; destruct m;
-  try destruct (inputEqDec i i0);
-  try destruct (outputEqDec o o0);
+  try destruct (inputEqDec t i i0);
+  try destruct (outputEqDec t o o0);
   try solve [left; congruence];
   try solve [right; congruence].
  Qed.
 
  (* Given a mapping from variables to values, a "worker function" computes a value *)
- Definition Env    := Var -> val.
- Definition Func t := Env -> t.
+ Definition Env    := Var -> val t.
+ Definition Func a := Env -> a.
 
-
- (* State labels *)
- Variable label : Type.
 
  (* Put the labels in the state type so we don't need dependent types or whatever *)
  Inductive State
    (* Pull from an input channel *)
-  := Pull    : input
+  := Pull    : input t
              (*some*) (*none*)
-            -> label -> label
+            -> label t -> label t
             -> State
    (* Release input value *)
-   | Release : input -> label
+   | Release : input t -> label t
             -> State
    (* Close input channel - I promise not to read again *)
-   | Close   : input -> label
+   | Close   : input t -> label t
             -> State
    (* Push f(env) to output channel *)
-   | Out     : output
-            -> Func val
-            -> label
+   | Out     : output t
+            -> Func  (val t)
+            -> label  t
             -> State
    (* Output channel is finished *)
-   | OutDone : output
-            -> label
+   | OutDone : output t
+            -> label  t
             -> State
    (* If f(env) *)
    | If      : Func bool
              (*then*) (*else*)
-            -> label -> label
+            -> label t -> label t
             -> State
    (* output's state = f(env) *)
-   | Update  : output
-            -> Func val
-            -> label
+   | Update  : output t
+            -> Func  (val t)
+            -> label  t
             -> State
    (* Goto*)
-   | Skip    : label
+   | Skip    : label  t
             -> State
    (* Nothing more to do *)
    | Done    : State.
 
- (* We need an initial label *)
- Variable initial : label.
+ (* Finally, each label needs a state *)
+ Variable stateOf : label t -> State.
 
- (* And each label needs a state *)
- Variable stateOf : label -> State.
 
 
 
@@ -107,19 +118,19 @@ Section Machine.
 
  (* We need some values to start the party *)
  Definition emptyEnv : Env
-  := fun _ => uninitialised.
+  := fun _ => uninitialised t.
 
  (* Each input channel needs a list of values, as does output *)
- Definition Inputs  := input  -> list val.
- Definition Outputs := output -> list val.
+ Definition Inputs  := input  t -> list (val t).
+ Definition Outputs := output t -> list (val t).
 
  (* Pull from an input *)
- Definition pull (i : input) (is : Inputs) : (Inputs * option val)
+ Definition pull (i : input t) (is : Inputs) : (Inputs * option (val t))
   := match is i with
      | [] 
         => (is, None)
      | (x::xs)
-        => (update _ _ inputEqDec i xs is, Some x)
+        => (update _ _ (inputEqDec t) i xs is, Some x)
      end.
 
  (* Initially all outputs are empty *)
@@ -127,10 +138,10 @@ Section Machine.
   := Map.empty _ _ [].
 
  (* Push to an output *)
- Definition push (o : output) (v : val) (os : Outputs) : Outputs
-  := update _ _ outputEqDec o (v :: os o) os.
+ Definition push (o : output t) (v : val t) (os : Outputs) : Outputs
+  := update _ _ (outputEqDec t) o (v :: os o) os.
 
- Definition STATE := (label * Inputs * Outputs * Env)%type.
+ Definition STATE := (label t * Inputs * Outputs * Env)%type.
 
  Definition run1 (r : STATE) : STATE
   := match r with
@@ -174,7 +185,7 @@ Section Machine.
      end.
 
 
- Inductive runs : STATE -> STATE -> Type
+ Inductive runs : STATE -> STATE -> Prop
  := RunDone   : forall l is os e
               , stateOf l = Done
              -> runs (l,is,os,e) (l,is,os,e)
@@ -182,10 +193,27 @@ Section Machine.
               , runs (run1 s) s'
              -> runs s s'.
 
- Inductive exec : Inputs -> Outputs -> Type
+ Inductive exec : Inputs -> Outputs -> Prop
   := Exec     : forall is l' is' os' e'
-              , runs (initial, is, initialOuts, emptyEnv)
+              , runs (initial t, is, initialOuts, emptyEnv)
                      (l', is', os', e')
              -> exec is os'.
+
+ Definition terminates
+              := forall is,
+              exists os,
+              exec is os.
+
+
+ (* but in order to prove termination of whole program,
+    probably need to show for all states *)
+ Definition terminates_all_states
+              := forall l is os e,
+              exists l' is' os' e',
+              runs (l, is, os, e) (l', is', os', e').
+
+ (* Termination variant?
+    Maybe something about, for each label L, whenever you get back to L
+    either lists will be shorter, or some variant on env will be smaller *)
 
 End Machine.
