proof/Merges/Map.v
@@ -6,6 +6,13 @@ Section Map.
  Definition EqDec  := forall (n m : K), { n = m } + { n <> m }.
  Hypothesis EqDec_ : forall (n m : K), { n = m } + { n <> m }.
 
+ Ltac eqdec :=
+  unfold EqDec in *; intros n m;
+  induction n; induction m;
+  try solve [left; congruence];
+  try solve [right; congruence].
+
+
  Definition Map := K -> V.
 
  Definition empty (v : V) : Map
